src/program_proof/simplefs/blockfs_proof.v
@@ -1,9 +1,11 @@
 From Perennial.program_proof Require Import proof_prelude.
+From Perennial.program_proof Require Import disk_prelude.
+
 From Goose.github_com Require Import tchajed.simplefs.filesys.
 
-From Perennial.program_proof Require Import disk_prelude.
 From Perennial.goose_lang.lib Require Import typed_slice.
 
+From Perennial.program_proof Require Import disk_lib.
 From Perennial.program_proof.simplefs Require Import
   inode_proof
   block_alloc_proof
@@ -74,18 +76,117 @@ current inode data. *)
 Definition bfile_ptsto γ i f: iProp _ :=
   ∃ ino, own_bfile γ i ino f.
 
-Definition own_blockFs (γ: blockfs_names) (l: loc) : iProp _ :=
+(* Note that [own_blockFs] exposes the exact logical state of the file system.
+It owns the entire disk, including all inode points-to facts, which permits
+looking up inodes without explicitly having ownership. *)
+Definition own_blockFs (γ: blockfs_names) (l: loc) (bfiles: gmap w64 block_file.t) : iProp _ :=
   ∃ (sb_l ba_l ia_l: loc),
-  "sb_l" ∷ l ↦[blockFs :: "sb"]□ #sb_l ∗
-  "d" ∷ l ↦[blockFs :: "d"]□ #() ∗
-  "ba_l" ∷ l ↦[blockFs :: "ba"]□ #ba_l ∗
-  "ia_l" ∷ l ↦[blockFs :: "ia"]□ #ia_l ∗
-  "Hauth" ∷ blockfs_auth γ ∗
-  ∃ (sb: superblockT),
-    "#sb" ∷ is_superblock (sb_var γ) sb_l sb ∗
-    "Hba" ∷ own_block_alloc (sb_var γ) ba_l ∗
-    "Hia" ∷ own_inode_alloc γ.(inode_var) ia_l ∗
-    "Hinodes" ∷ inode_auth γ.(inode_var)
+  "#sb_l" ∷ l ↦[blockFs :: "sb"]□ #sb_l ∗
+  "#d" ∷ l ↦[blockFs :: "d"]□ #() ∗
+  "#ba_l" ∷ l ↦[blockFs :: "ba"]□ #ba_l ∗
+  "#ia_l" ∷ l ↦[blockFs :: "ia"]□ #ia_l ∗
+  (* "Hauth" ∷ blockfs_auth γ ∗ *)
+  ∃ (sb: superblockT), "#sb" ∷ is_superblock (sb_var γ) sb_l sb ∗
+  "Hba" ∷ own_block_alloc (sb_var γ) ba_l ∗
+  "Hinodes" ∷ inode_auth γ.(inode_var) ∗
+  ∃ free,
+  "%Hinum_complete" ∷ ⌜∀ inum, sb_valid_inum sb inum →
+                                 inum ∈ free ∨ inum ∈ dom bfiles⌝ ∗
+  "Hia" ∷ own_inode_alloc γ.(inode_var) ia_l free ∗
+  "Hfiles" ∷ [∗ map] inum↦f ∈ bfiles, bfile_ptsto γ inum f
 .
+
+Definition sb_disk_ptsto sb : iProp _ :=
+    0 d↦ list_to_block (sb_encode sb).
+Definition sb_zero_data_bitmap sb : iProp _ :=
+    sb_data_bitmap_start sb d↦∗ (replicate (uint.nat sb.(data_bitmap_blocks)) block0).
+Definition sb_data_blocks sb: iProp _ :=
+    ∃ bs, ⌜length bs = uint.nat sb.(data_blocks)⌝ ∗ sb_data_start sb d↦∗ bs.
+
+Theorem wp_zeroDisk (sz : u64) bs :
+  {{{ 0 d↦ bs ∗ ⌜length bs = uint.nat sz⌝ }}}
+    zeroDisk #() #sz
+  {{{ γsb (l : loc) sb, RET #l;
+      is_superblock γsb l sb ∗
+      sb_disk_ptsto sb ∗ sb_zero_data_bitmap sb ∗ sb_data_blocks sb ∗
+      sb_inode_start sb d↦∗ (replicate (uint.nat sb.(inode_blocks)) block0)
+  }}}.
+Proof.
+  (*@ func zeroDisk(d disk.Disk, sz uint64) *superblock.Superblock {          @*)
+  (*@     sb := superblock.InitSuperblock(sz)                                 @*)
+  (*@     d.Write(0, sb.Encode())                                             @*)
+  (*@                                                                         @*)
+  (*@     zero_blk := make(disk.Block, disk.BlockSize)                        @*)
+  (*@     for i := uint64(0); i < sb.InodeBlocks; i++ {                       @*)
+  (*@         d.Write(sb.InodeStart()+i, zero_blk)                            @*)
+  (*@     }                                                                   @*)
+  (*@     for i := uint64(0); i < sb.DataBitmapBlocks; i++ {                  @*)
+  (*@         d.Write(sb.DataBitmapStart()+i, zero_blk)                       @*)
+  (*@     }                                                                   @*)
+  (*@     // data does not have to be zeroed                                  @*)
+  (*@     return sb                                                           @*)
+  (*@ }                                                                       @*)
+Admitted.
+
+Definition root_ino: inode_rep.t :=
+  inode_rep.mk inodeType.dirType (W64 0) (W32 493) (vreplicate _ (W32 0)).
+
+Definition init_inodes (sb: superblockT) :=
+  <[W64 1 := root_ino]> (init_inode_map (uint.nat sb.(inode_blocks) * 32)%nat).
+
+(* the on-disk facts for an initialized file system *)
+Definition init_fs γ sb: iProp _ :=
+    "sb_disk" ∷ sb_disk_ptsto sb ∗
+    "data_bitmaps" ∷ sb_zero_data_bitmap sb ∗
+    "inodes" ∷
+      ([∗ map] inum↦ino ∈ init_inodes sb,
+        inode_ptsto γ.(inode_var) inum ino) ∗
+    "data_blocks" ∷ sb_data_blocks sb.
+
+Theorem wp_mkBlockFs (sz : w64) (bs: list Block) :
+  {{{ 0 d↦∗ bs ∗ ⌜length bs = uint.nat sz⌝ }}}
+    mkBlockFs #() #sz
+  {{{ γ sb, RET #(); init_fs γ sb
+  }}}.
+Proof.
+  (*@ func mkBlockFs(d disk.Disk, sz uint64) {                                @*)
+  (*@     sb := superblock.InitSuperblock(sz)                                 @*)
+  (*@     d.Write(0, sb.Encode())                                             @*)
+  (*@                                                                         @*)
+  (*@     zero_blk := make(disk.Block, disk.BlockSize)                        @*)
+  (*@     for i := uint64(0); i < sb.InodeBlocks; i++ {                       @*)
+  (*@         d.Write(sb.InodeStart()+i, zero_blk)                            @*)
+  (*@     }                                                                   @*)
+  (*@     for i := uint64(0); i < sb.DataBitmapBlocks; i++ {                  @*)
+  (*@         d.Write(sb.DataBitmapStart()+i, zero_blk)                       @*)
+  (*@     }                                                                   @*)
+  (*@     // data does not have to be zeroed                                  @*)
+  (*@                                                                         @*)
+  (*@     root_inode := inode.NewInode(simplefs.DirType)                      @*)
+  (*@     root_inode.SetMeta(inode.Meta{Mode: 0o755})                         @*)
+  (*@     root_inode.Write(d, sb, simplefs.ROOT_INUM)                         @*)
+  (*@ }                                                                       @*)
+Admitted.
+
+Definition root_bfile: block_file.t :=
+  block_file.mk inodeType.dirType (W64 0) (W32 493) (vreplicate _ block0).
+
+(* only specified for a newly created file system *)
+Theorem wp_loadBlockFs γ sb :
+  {{{ init_fs γ sb }}}
+    loadBlockFs #()
+  {{{ (l : loc), RET #l;
+      is_sb (sb_var γ) sb ∗
+      own_blockFs γ l {[ W64 1 := root_bfile ]}
+  }}}.
+Proof.
+  (*@ func loadBlockFs(d disk.Disk) *blockFs {                                @*)
+  (*@     sb := superblock.LoadSuperblock(d)                                  @*)
+  (*@     ba := alloc.NewBlockAllocator(d, sb)                                @*)
+  (*@     ia := alloc.NewInodeAllocator(d, sb)                                @*)
+  (*@     return &blockFs{sb: sb, d: d, ba: ba, ia: ia}                       @*)
+  (*@ }                                                                       @*)
+Admitted.
+
 
 End proof.
